src/high/modalities/post_fence_sync_advanced.v
@@ -1,0 +1,197 @@
+From iris.proofmode Require Import proofmode monpred.
+From iris_named_props Require Import named_props.
+
+From self Require Import solve_view_le.
+From self.base Require Import generational_resources primitive_laws.
+From self.high Require Import wrappers protocol locations.
+From self.high.lib Require Import abstract_state.
+From self.high.modalities Require Import fence.
+
+From self.high Require Export dprop.
+
+Set Default Proof Using "Type*".
+
+Section post_fence_sync.
+  Context `{!nvmBaseGS Σ Ω, !nvmHighGS Σ Ω}.
+  Implicit Types (ℓ : loc) (P Q: dProp Σ).
+  (* For every location we [flush], we will keep the follow tuple,
+   * - [ℓ], the location
+   * - [σ], the abstract state we flush,
+   * - [σ_xchg], the "exchange" state we want to extract resources from,
+   * - [seen ℓ σ_xchg], so that we have the necessary view,
+   * and we also keep enough resource to make three consecutive exchanges/updates with
+   * the protocol in the future and obtain final post condition [R] (when we [flush_sync]),
+   * - [<obj> p_read σ v -∗ □ <obj> P], for getting some basic facts about the physical value,
+   * - [P -∗ <obj> (p_pers σ_old v_old ==∗ <obj> Q ∗ p_pers σ v)] roughly, for the persistent state update,
+   * - [Q -∗ <obj> (p_read σ_xchg v_xchg ==∗ R ∗ p_read σ_xchg v_xchg)] for the read only exchange. *)
+
+  Definition exchange_3 `{AbstractState ST} ℓ (σ_xchg: ST) (prot: LocationProtocol ST) Q: dProp Σ :=
+    ∀ v_xchg, <obj> (prot.(p_read) σ_xchg v_xchg ==∗ Q ∗ prot.(p_read) σ_xchg v_xchg).
+
+  (* TODO: include the other case as well *)
+  Definition exchange_2 `{AbstractState ST} ℓ (σ_xchg σ: ST) v (prot: LocationProtocol ST) Q: dProp Σ :=
+    ∀ σ_old v_old,
+    <obj> ((⌜ σ_old ⊑ σ ⌝ -∗ prot.(p_pers) σ_old v_old ==∗
+           prot.(p_pers) σ v ∗ exchange_3 ℓ σ_xchg prot Q) ∧
+           (⌜ σ ⊑ σ_old ⌝ -∗ prot.(p_pers) σ_old v_old ==∗
+           prot.(p_pers) σ_old v_old ∗ exchange_3 ℓ σ_xchg prot Q)).
+
+  Definition exchange_1 `{AbstractState ST} ℓ (σ_xchg σ: ST) (prot: LocationProtocol ST) Q: dProp Σ :=
+    ∀ v,
+    <obj> (prot.(p_read) σ v -∗ prot.(p_read) σ v ∗ exchange_2 ℓ σ_xchg σ v prot Q).
+
+  Record FlushInfo := MkFlushInfo {
+    fi_ℓ: loc;
+    fi_ST: Type;
+    fi_ST_eqdec :> EqDecision fi_ST;
+    fi_ST_countable :> Countable fi_ST;
+    fi_ST_is_abstract :> AbstractState fi_ST;
+    fi_prot: LocationProtocol fi_ST;
+    fi_prot_conds :> ProtocolConditions fi_prot;
+    fi_σ: fi_ST;
+    fi_σ_xchg: fi_ST;
+    fi_post: dProp Σ
+  }.
+
+  #[local] Definition internal_flush_lb `{AbstractState ST} ℓ (prot: LocationProtocol ST) (s : ST) : dProp Σ :=
+    ∃ (t : nat) offset,
+      "#lbBase" ∷ lb_base ℓ prot offset t s ∗
+      (* this assertion is only ever to be used internally, we can safely assert over
+       *  about buffer views. *)
+      "%haveBV" ∷ have_thread_view (∅, ∅, {[ ℓ := MaxNat (t - offset) ]}).
+
+  Program Definition post_fence_sync_advanced
+    (P : dProp Σ) : dProp Σ :=
+    MonPred (λ TV,
+      ∃ (fi_list: list FlushInfo),
+        ([∗ list] fi ∈ fi_list,
+           ⎡ is_at_loc fi.(fi_ℓ) ⎤ ∗
+           know_protocol fi.(fi_ℓ) fi.(fi_prot) ∗
+           (* this can probably be promoted to [flush_lb], but doens't seem necessary? *)
+           internal_flush_lb fi.(fi_ℓ) fi.(fi_prot) fi.(fi_σ) ∗
+           seen_state fi.(fi_ℓ) fi.(fi_prot) fi.(fi_σ_xchg) ∗
+           exchange_1 fi.(fi_ℓ) fi.(fi_σ_xchg) fi.(fi_σ) fi.(fi_prot) fi.(fi_post))
+          TV ∗
+        ((persisted (buffer_view TV)) -∗
+         (([∗ list] fi ∈ fi_list, fi.(fi_post)) -∗ P)
+           (store_view TV, (flush_view TV ⊔ buffer_view TV), buffer_view TV))
+      )%I _.
+  Next Obligation.
+    intros P. intros [[??]?] [[??]?] [[??]?]. simpl.
+    assert (g0 ⊔ g1 ⊑ g3 ⊔ g4). { solve_proper. }
+    iIntros "(%fi_list & Hfi & P)".
+    iExists fi_list.
+    iSplitL "Hfi".
+    - iApply monPred_mono; last done.
+      solve_view_le.
+    - iIntros "pers".
+      iPoseProof (persisted_anti_mono with "pers") as "pers";
+        (* use the special reasoning to figure out the view automatically. *)
+        last iSpecialize ("P" with "pers"); first done.
+      iApply monPred_mono; last done.
+      solve_view_le.
+  Qed.
+End post_fence_sync.
+
+Notation "'<FS>' P" :=
+  (post_fence_sync_advanced P) (at level 20, right associativity) : bi_scope.
+
+Section lemmas.
+  Context `{!nvmBaseGS Σ Ω, !nvmHighGS Σ Ω}.
+  Implicit Types (ℓ : loc) (P Q: dProp Σ).
+
+  Lemma post_fenc_sync_advanced_post_fence_sync P :
+    <fence_sync> P -∗ <FS> P.
+  Proof.
+    iModel. simpl.
+    iIntros "P".
+    iExists []. simpl.
+    rewrite left_id.
+    iFrame.
+    done.
+  Qed.
+
+  Lemma post_fence_sync_advanced_mono P Q : (P ⊢ Q) → <FS> P ⊢ <FS> Q.
+  Proof.
+    intros Hi. iModel. simpl.
+    iIntros "(%fi_list & exchanges & P)".
+    iExists fi_list.
+    rewrite -Hi.
+    iFrame.
+  Qed.
+
+  Lemma post_fence_sync_advanced_intro P : P ⊢ <FS> P.
+  Proof.
+    iModel. destruct TV as [[??]?]. simpl.
+    iIntros "P".
+    iExists []. simpl.
+    iSplitR; first done.
+    iIntros "pers".
+    rewrite left_id.
+    iApply (monPred_mono with "P"). repeat split; auto using view_le_l.
+  Qed.
+
+  Lemma post_fence_sync_advanced_emp : (emp : dProp Σ) ⊢ <FS> emp.
+  Proof. apply post_fence_sync_advanced_intro. Qed.
+
+  Lemma post_fence_sync_and P Q : <FS> (P ∧ Q) ⊣⊢ <FS> P ∧ <FS> Q.
+  Proof.
+  Abort.
+
+  Lemma post_fece_sync_advanced_sep P Q:
+    post_fence_sync_advanced P ∗ post_fence_sync_advanced Q ⊢ (post_fence_sync_advanced (P ∗ Q)).
+  Proof.
+    iModel.
+    destruct TV as [[SV PV] BV].
+    iIntros "[P Q]".
+    rewrite /post_fence_sync_advanced /=.
+    iDestruct "P" as (P_list) "[P_exchanges Ppost]".
+    iDestruct "Q" as (Q_list) "[Q_exchanges Qpost]".
+    iExists (P_list ++ Q_list).
+    rewrite ?monPred_at_big_sepL.
+    iDestruct (big_sepL_app with "[$P_exchanges $Q_exchanges]") as "exchanges".
+    iFrame "exchanges".
+    rewrite big_sepL_app.
+    rewrite ?monPred_at_wand.
+    iIntros "#persisted" ([[SV' PV'] BV'] [[? ?] ?]) "[Pfi_post Qfi_post]".
+    iSpecialize ("Ppost" with "[$]").
+    iDestruct ("Ppost" with "[] Pfi_post") as "$".
+    { iPureIntro. solve_view_le. }
+    iSpecialize ("Qpost" with "[$]").
+    iDestruct ("Qpost" with "[] Qfi_post") as "$".
+    { iPureIntro. solve_view_le. }
+  Qed.
+
+  Lemma post_fence_sync_advanced_intuitionistically_2 P : □ <FS> P ⊢ <FS> □ P.
+  Proof.
+    iModel. simpl.
+    iIntros "(%fi_list & #exchanges & #P)".
+    iExists fi_list.
+    iFrame "exchanges".
+    iIntros "#persisted".
+    iSpecialize ("P" with "persisted").
+    rewrite ?monPred_at_wand.
+    iIntros (TV' ?) "fi_post".
+    iSpecialize ("P" with "[//] fi_post").
+  Abort.
+End lemmas.
+
+Section Tests.
+  Context `{!nvmBaseGS Σ Ω, !nvmHighGS Σ Ω, !PerennialG Σ, AbstractState ST}.
+  
+  Variables (ℓ : loc) (prot: LocationProtocol ST) (σ σ_xchg: ST) (P: iProp Σ) (Q: dProp Σ).
+
+  (* just need to make sure [P] survives until last exchange *)
+  Example embed_into_exchange_3:
+    ⎡ P ⎤ ⊢ exchange_1 ℓ σ σ_xchg prot Q.
+  Proof.
+    rewrite /exchange_1 /exchange_2 /exchange_3.
+    iIntros "P" (v) "!> $".
+    iIntros (σ_old v_old) "!>".
+    iSplit.
+    - admit.
+    - iIntros (?) "$ !>".
+      iIntros (v_xchg) "!> $".
+      iClear "P".
+  Abort.
+End Tests.
